add plf content here

plf/.coqdeps.d
@@ -1,6 +1,14 @@
 Equiv.vo Equiv.glob Equiv.v.beautified: Equiv.v Maps.vo Imp.vo
 Equiv.vio: Equiv.v Maps.vio Imp.vio
+Hoare.vo Hoare.glob Hoare.v.beautified: Hoare.v Maps.vo Imp.vo
+Hoare.vio: Hoare.v Maps.vio Imp.vio
+Hoare2.vo Hoare2.glob Hoare2.v.beautified: Hoare2.v Maps.vo Hoare.vo Imp.vo
+Hoare2.vio: Hoare2.v Maps.vio Hoare.vio Imp.vio
+HoareAsLogic.vo HoareAsLogic.glob HoareAsLogic.v.beautified: HoareAsLogic.v Imp.vo Hoare.vo
+HoareAsLogic.vio: HoareAsLogic.v Imp.vio Hoare.vio
 Imp.vo Imp.glob Imp.v.beautified: Imp.v Maps.vo
 Imp.vio: Imp.v Maps.vio
 Maps.vo Maps.glob Maps.v.beautified: Maps.v
 Maps.vio: Maps.v
+Smallstep.vo Smallstep.glob Smallstep.v.beautified: Smallstep.v Maps.vo Imp.vo
+Smallstep.vio: Smallstep.v Maps.vio Imp.vio
