plf/Hoare.v
@@ -5,6 +5,7 @@ From Coq Require Import Arith.Arith.
 From Coq Require Import Arith.EqNat.
 From Coq Require Import Arith.PeanoNat. Import Nat.
 From Coq Require Import omega.Omega.
+From Coq Require Import FunctionalExtensionality.
 From PLF Require Import Imp.
 
 Definition Assertion := state -> Prop.
@@ -68,3 +69,235 @@ Definition assn_sub X a P: Assertion :=
 
 Notation "P [ X |-> a ]" := (assn_sub X a P)
   (at level 10, X at next level).
+
+
+Theorem hoare_asgn : forall Q X a,
+  {{Q [X |-> a]}} X ::= a {{Q}}.
+Proof.
+  unfold hoare_triple.
+  intros Q X a st st' HE HQ.
+  inversion HE. subst.
+  unfold assn_sub in HQ. assumption. Qed.
+
+
+Theorem hoare_asgn_fwd:
+  forall m a P,
+    {{fun st => P st /\ st X = m}}
+      X ::= a
+    {{fun st => P (X !-> m ; st) /\
+             st X = aeval (X !-> m ; st) a}}.
+Proof.
+  unfold hoare_triple.
+  intros.
+  inversion H; subst.
+  destruct H0.
+  rewrite t_update_shadow.
+  rewrite <- H1. rewrite t_update_same.
+  auto.
+Qed.
+
+Theorem hoare_consequence_pre : forall (P P' Q : Assertion) c,
+  {{P'}} c {{Q}} ->
+  P ->> P' ->
+  {{P}} c {{Q}}.
+Proof.
+  intros P P' Q c Hhoare Himp.
+  intros st st' Hc HP.
+  apply (Hhoare st st'). assumption.
+  apply Himp. assumption.
+Qed.
+
+Theorem hoare_consequence_post : forall (P Q Q' : Assertion) c,
+  {{P}} c {{Q'}} ->
+  Q' ->> Q ->
+  {{P}} c {{Q}}.
+Proof.
+  intros P Q Q' c Hhoare Himp.
+  intros st st' Hc HP.
+  apply Himp.
+  apply (Hhoare st st').
+  assumption. assumption. Qed.
+
+Example hoare_asgn_example1 :
+  {{fun st => True}} X ::= 1 {{fun st => st X = 1}}.
+Proof.
+  apply hoare_consequence_pre
+    with (P' := (fun st => st X = 1) [X |-> 1]).
+  apply hoare_asgn.
+  intros st H.
+  unfold assn_sub. auto.
+Qed.
+
+Theorem hoare_consequence : forall(P P' Q Q' : Assertion) c,
+  {{P'}} c {{Q'}} ->
+  P ->> P' ->
+  Q' ->> Q ->
+  {{P}} c {{Q}}.
+Proof.
+  intros P P' Q Q' c Hht HPP' HQ'Q.
+  apply hoare_consequence_pre with (P' := P').
+  apply hoare_consequence_post with (Q' := Q').
+  assumption. assumption. assumption. Qed.
+
+Theorem hoare_skip : forall P,
+     {{P}} SKIP {{P}}.
+Proof.
+  intros P st st' H HP. inversion H. subst.
+  assumption. Qed.
+
+Theorem hoare_seq : forall P Q R c1 c2,
+     {{Q}} c2 {{R}} ->
+     {{P}} c1 {{Q}} ->
+     {{P}} c1;;c2 {{R}}.
+Proof.
+  intros P Q R c1 c2 H1 H2 st st' H12 Pre.
+  inversion H12; subst.
+  apply (H1 st'0 st'); try assumption.
+  apply (H2 st st'0); assumption. Qed.
+
+Example hoare_asgn_example3 : forall a n,
+  {{fun st => aeval st a = n}}
+  X ::= a;; SKIP
+  {{fun st => st X = n}}.
+Proof.
+  intros a n. eapply hoare_seq.
+  - (* right part of seq *)
+    apply hoare_skip.
+  - (* left part of seq *)
+    eapply hoare_consequence_pre. apply hoare_asgn.
+    intros st H. subst. reflexivity.
+Qed.
+
+Definition swap_program : com :=
+  Z ::= AId X ;; X ::= AId Y ;; Y ::= AId Z.
+
+Theorem swap_ex:
+  {{fun st => st X <= st Y}}
+  swap_program
+  {{fun st => st Y <= st X}}.
+Proof.
+  eapply hoare_seq. eapply hoare_seq.
+  - eapply hoare_consequence_pre.
+    apply hoare_asgn.
+    intros st H. eauto.
+  - eapply hoare_consequence_pre.
+    apply hoare_asgn.
+    intros st H. eauto.
+  - eapply hoare_consequence_pre.
+    apply hoare_asgn.
+    intros st H. eauto.
+Qed.
+
+(* lift of bool *)
+Definition bassn b: Assertion :=
+  fun st => (beval st b = true).
+
+Lemma bexp_eval_true : forall b st,
+    beval st b = true -> (bassn b) st.
+Proof.
+  intros. unfold bassn. apply H.
+Qed.
+
+Lemma bexp_eval_false : forall b st,
+    beval st b = false -> not ((bassn b) st).
+Proof.
+  intros. unfold bassn.
+  rewrite H. auto. Qed.
+
+Hint Unfold bassn.
+Theorem hoare_if : forall P Q b c1 c2,
+  {{fun st => P st /\ bassn b st}} c1 {{Q}} ->
+  {{fun st => P st /\ not (bassn b st)}} c2 {{Q}} ->
+  {{P}} TEST b THEN c1 ELSE c2 FI {{Q}}.
+Proof.
+  intros.
+  intros st st' HE HP.
+  inversion HE; subst.
+  apply (H st); auto.
+  apply (H0 st); auto.
+  split. assumption. unfold bassn.
+  rewrite H6. auto.
+Qed.
+
+Example if_example :
+    {{fun st => True}}
+  TEST X = 0
+    THEN Y ::= 2
+    ELSE Y ::= X + 1
+  FI
+    {{fun st => st X <= st Y}}.
+Proof.
+  (* WORKED IN CLASS *)
+  apply hoare_if.
+  - (* Then *)
+    eapply hoare_consequence_pre. apply hoare_asgn.
+    unfold bassn, assn_sub, t_update, assert_implies.
+    simpl. intros st [_ H].
+    apply eqb_eq in H.
+    rewrite H. omega.
+  - (* Else *)
+    eapply hoare_consequence_pre. apply hoare_asgn.
+    unfold assn_sub, t_update, assert_implies.
+    simpl; intros st _. omega.
+Qed.
+
+Theorem if_minus_plus :
+  {{fun st => True}}
+  TEST X <= Y
+    THEN Z ::= Y - X
+    ELSE Y ::= X + Z
+  FI
+  {{fun st => st Y = st X + st Z}}.
+Proof.
+  apply hoare_if.
+  - eapply hoare_consequence_pre.
+    apply hoare_asgn.
+    unfold bassn, assn_sub, assert_implies, t_update.
+    simpl; intros st [_ Ht].
+    Search (_ = _ + (_ - _)).
+    Search (_ <=? _ = true).
+    apply leb_le in Ht.
+    apply le_plus_minus. assumption.
+  - eapply hoare_consequence_pre.
+    apply hoare_asgn.
+    unfold bassn, assn_sub, assert_implies, t_update.
+    simpl. auto.
+Qed.
+
+Theorem hoare_while : forall P b c,
+  {{fun st => P st /\ bassn b st}} c {{P}} ->
+  {{P}} WHILE b DO c END {{fun st => P st /\ not (bassn b st)}}.
+Proof.
+  intros P b c Hhoare st st' He HP.
+  remember (WHILE b DO c END)%imp as wcom.
+  induction He;
+    try (inversion Heqwcom); subst.
+  - split. assumption. unfold bassn.
+    apply bexp_eval_false. assumption.
+  - apply IHHe2. assumption.
+    apply (Hhoare st). assumption.
+    split. assumption. apply bexp_eval_true. assumption.
+Qed.
+
+Theorem always_loop_hoare : forall P Q,
+  {{P}} WHILE true DO SKIP END {{Q}}.
+Proof.
+  (* WORKED IN CLASS *)
+  intros P Q.
+  apply hoare_consequence_pre with (P' := fun st : state => True).
+  eapply hoare_consequence_post.
+  apply hoare_while.
+  - (* Loop body preserves invariant *)
+    apply hoare_post_true. intros st. apply I.
+  - (* Loop invariant and negated guard imply postcondition *)
+    simpl. intros st [Hinv Hguard].
+    exfalso. apply Hguard. reflexivity.
+  - (* Precondition implies invariant *)
+    intros st H. constructor. Qed.
+
+
+
+
+
+
+
