plf/Types.v
@@ -1,0 +1,144 @@
+Set Warnings "-notation-overridden,-parsing".
+From Coq Require Import Arith.Arith.
+From PLF Require Import Maps.
+From PLF Require Import Imp.
+From PLF Require Import Smallstep.
+Hint Constructors multi.
+
+Inductive tm : Type :=
+  | tru : tm
+  | fls : tm
+  | test : tm -> tm -> tm -> tm
+  | zro : tm
+  | scc : tm -> tm
+  | prd : tm -> tm
+  | iszro : tm -> tm.
+
+Inductive bvalue : tm -> Prop :=
+  | bv_tru : bvalue tru
+  | bv_fls : bvalue fls.
+Inductive nvalue : tm -> Prop :=
+  | nv_zro : nvalue zro
+  | nv_scc : forall t, nvalue t -> nvalue (scc t).
+Definition value (t : tm) := bvalue t \/ nvalue t.
+Hint Constructors bvalue nvalue.
+Hint Unfold value.
+Hint Unfold update.
+
+Reserved Notation "t1 '-->' t2" (at level 40).
+Inductive step : tm -> tm -> Prop :=
+  | ST_TestTru : forall t1 t2,
+      (test tru t1 t2) --> t1
+  | ST_TestFls : forall t1 t2,
+      (test fls t1 t2) --> t2
+  | ST_Test : forall t1 t1' t2 t3,
+      t1 --> t1' ->
+      (test t1 t2 t3) --> (test t1' t2 t3)
+  | ST_Scc : forall t1 t1',
+      t1 --> t1' ->
+      (scc t1) --> (scc t1')
+  | ST_PrdZro :
+      (prd zro) --> zro
+  | ST_PrdScc : forall t1,
+      nvalue t1 ->
+      (prd (scc t1)) --> t1
+  | ST_Prd : forall t1 t1',
+      t1 --> t1' ->
+      (prd t1) --> (prd t1')
+  | ST_IszroZro :
+      (iszro zro) --> tru
+  | ST_IszroScc : forall t1,
+       nvalue t1 ->
+      (iszro (scc t1)) --> fls
+  | ST_Iszro : forall t1 t1',
+      t1 --> t1' ->
+      (iszro t1) --> (iszro t1')
+where "t1 '-->' t2" := (step t1 t2).
+Hint Constructors step.
+
+Notation step_normal_form := (normal_form step).
+Definition stuck (t : tm) : Prop :=
+  step_normal_form t /\ not (value t).
+Hint Unfold stuck.
+
+(* some invalid exp *)
+Example some_term_is_stuck :
+  exists t, stuck t.
+Proof.
+  exists (prd tru). unfold stuck.
+  split. intros contra.
+  destruct contra. inversion H; subst.
+  inversion H1.
+  intros contra.
+  destruct contra; inversion H.
+Qed.
+
+Lemma value_is_nf : forall t,
+  value t -> step_normal_form t.
+Proof.
+  intros t Hval contra; inversion Hval;subst;
+    induction H; inversion contra; subst;
+      try inversion H0;subst;
+        eauto;
+        try inversion H;subst.
+Qed.
+
+Hint Resolve value_is_nf.
+
+Theorem step_deterministic:
+  deterministic step.
+Proof with eauto.
+Admitted.
+
+Inductive ty : Type :=
+  | Bool : ty
+  | Nat : ty.
+Reserved Notation "'|-' t '∈' T" (at level 40).
+
+Inductive has_type : tm -> ty -> Prop :=
+  | T_Tru :
+       |- tru ∈ Bool
+  | T_Fls :
+       |- fls ∈ Bool
+  | T_Test : forall t1 t2 t3 T,
+       |- t1 ∈ Bool ->
+       |- t2 ∈ T ->
+       |- t3 ∈ T ->
+       |- test t1 t2 t3 ∈ T
+  | T_Zro :
+       |- zro ∈ Nat
+  | T_Scc : forall t1,
+       |- t1 ∈ Nat ->
+       |- scc t1 ∈ Nat
+  | T_Prd : forall t1,
+       |- t1 ∈ Nat ->
+       |- prd t1 ∈ Nat
+  | T_Iszro : forall t1,
+       |- t1 ∈ Nat ->
+       |- iszro t1 ∈ Bool
+where "'|-' t '∈' T" := (has_type t T).
+
+Hint Constructors has_type.
+
+Example has_type_1 :
+  |- test fls zro (scc zro) ∈ Nat.
+Proof.
+  apply T_Test.
+    - apply T_Fls.
+    - apply T_Zro.
+    - apply T_Scc.
+       + apply T_Zro.
+Qed.
+
+Example has_type_not :
+  not( |- test fls zro tru ∈ Bool ).
+Proof.
+  intros Contra. solve_by_inverts 2. Qed.
+
+Example scc_hastype_nat__hastype_nat : forall t,
+  |- scc t ∈ Nat ->
+  |- t ∈ Nat.
+Proof.
+  intros. inversion H. assumption.
+Qed.
+
